Some better organization

MergeSort.v
@@ -1,94 +1,15 @@
-(** Sorting Algorithms:*)
+From Sorting Require Import SortingHeader.
 
-From Stdlib Require Import List Arith.
-From Sorting Require Import Tactics.
-From Corelib Require Import Program.Wf.
-From Equations Require Import Equations.
-
-Import ListNotations.
-
-(* Today we will be covering sorting algorithms and proving their correctness. 
-
-First, we must define what it means for a list to be sorted. We will use the following abstract definition: "a list is sorted if each element is less than or equal to the next element in the list."
-*)
-
-Inductive sorted : list nat -> Prop :=
-(* The empty list is sorted *)
-| sorted_nil : sorted []
-(* A single-element list is sorted *)
-| sorted_singleton : forall x, sorted [x]
-(* If the head "x" is less than or equal to the head of "y :: l" (i.e. "y"), and "y :: l" is sorted, then the whole list is sorted *)
-| sorted_cons : forall x y l, 
-    x <= y -> 
-    sorted (y :: l) -> 
-    sorted (x :: y :: l).
-
-Theorem sorted_spec : forall h t,
-  sorted (h :: t) <-> ((forall x, In x t -> h <= x) /\ sorted t).
-Proof.
-  split; ff.
-  - prep_induction H.
-    induction H; ff.
-    * split; ff.
-      econstructor.
-    * pp (IHsorted _ _ eq_refl).
-      clear IHsorted.
-      ff.
-      split; ff.
-      pp (H1 _ H4).
-      lia.
-  - prep_induction H0.
-    induction H0; ff.
-    * econstructor.
-    * econstructor; ff.
-      econstructor.
-    * assert (sorted (x :: y :: l)). {
-        econstructor; ff.
-      }
-      econstructor; ff.
-Qed.
-
-
-(* We have established what it means to be sorted, but further we need to establish an overall theorem of "correctness" for a sorting algorithm.
-It is not simply enough to say that the output list is sorted; we must also ensure that the output list is a permutation of the input list.
-
-While this is certainly viable, I want to do something a little simpler than fully defining "permutation" here. 
-Instead, we will define a function that "counts the occurrences of an element in a list", and then we will prove that the count of each element in the input list is the same as the count of that element in the output list.
-*)
-
-Fixpoint count (x : nat) (l : list nat) : nat :=
-  match l with
-  | [] => 0
-  | h :: t => if Nat.eqb x h then S (count x t) else count x t
-  end.
-
-Lemma count_app : forall x l1 l2,
-  count x (l1 ++ l2) = count x l1 + count x l2.
-Proof.
-  induction l1; destruct l2; ff l.
-Qed.
-
-Program Fixpoint list_sync_ind_same {A : Type} (P : (list A * list A) -> Prop) 
-    (f_nil_l : forall r, P (nil, r))
-    (f_nil_r : forall l, P (l, nil))
-    (f_cons  : forall h1 h2 t1 t2, P (t1, t2) -> P (h1 :: t1, h2 :: t2))
-    (lp : (list A * list A))
-    {measure (length (fst lp) + length (snd lp))}
-    : P lp :=
-  match lp with
-  | (nil, r) => f_nil_l r
-  | (l, nil) => f_nil_r l
-  | (h1 :: t1, h2 :: t2) => 
-    f_cons h1 h2 t1 t2 
-      (list_sync_ind_same P f_nil_l f_nil_r f_cons (t1, t2))
-  end.
+Equations merge (l1 l2 : list nat) : list nat by wf (length l1 + length l2) :=
+  merge nil l2 := l2;
+  merge l1 nil := l1;
+  merge (h1 :: t1) (h2 :: t2) :=
+    if h1 <=? h2 
+    then h1 :: merge t1 (h2 :: t2)
+    else h2 :: merge (h1 :: t1) t2.
 Next Obligation.
   lia.
-Qed.
-Next Obligation.
-  eapply measure_wf.
-  eapply well_founded_ltof.
-Qed.
+Defined.
 
 Program Fixpoint list_sync_ind {A : Type} (P : (list A * list A) -> Prop) 
     (f_nil_l : forall r, P (nil, r))
@@ -115,795 +36,299 @@ Next Obligation.
   eapply well_founded_ltof.
 Qed.
 
-(* As a bonus lemma, we could prove this notion equivalent to that of a permutation: all permutations of a list have the same element counts <=> all lists with the same element counts are permutations of each other. *)
-Inductive permutation : list nat -> list nat -> Prop :=
-| perm_nil: permutation [] []
-| perm_skip x l l' : permutation l l' -> permutation (x::l) (x::l')
-| perm_swap x y l : permutation (y::x::l) (x::y::l)
-| perm_trans l l' l'' :
-    permutation l l' -> permutation l' l'' -> permutation l l''.
-
-Lemma perm_refl : forall l,
-  permutation l l.
+Lemma merge_in : forall l1 l2 x,
+  In x (merge l1 l2) <-> In x l1 \/ In x l2.
 Proof.
-  induction l; ff; econstructor; ff.
+  intros l1 l2.
+  pp (@list_sync_ind nat (fun lp => forall x : nat, In x (merge (fst lp) (snd lp)) <-> In x (fst lp) \/ In x (snd lp))).
+  simpl in *.
+  specialize H with (lp := (l1, l2)).
+  simpl in *.
+  eapply H; ff; clear H.
+  - ltac1:(autorewrite with merge in * ); destruct l; ff.
+  - ltac1:(autorewrite with merge in * ); destruct l; ff.
+  - ltac1:(autorewrite with merge in * ); ff.
+    * rewrite H1 in H; ff.
+    * rewrite H0 in H; ff.
+    Show Proof.
+    Print Assumptions merge_equation_3.
+  - ltac1:(autorewrite with merge in * ); ff.
+    * erewrite H1; ff.
+    * erewrite H0; ff.
 Qed.
+Print Assumptions merge_in.
 
-Lemma perm_sym : forall l1 l2,
-  permutation l1 l2 ->
-  permutation l2 l1.
+Theorem merge_sorted : forall l1 l2,
+  sorted l1 ->
+  sorted l2 ->
+  sorted (merge l1 l2).
 Proof.
-  intros.
-  induction H; try (econstructor; ff; fail).
+  intros l1 l2.
+  pp (@list_sync_ind nat (fun lp => sorted (fst lp) -> sorted (snd lp) -> sorted (merge (fst lp) (snd lp)))).
+  simpl in *.
+  specialize H with (lp := (l1, l2)).
+  simpl in *.
+  eapply H; ff; clear H.
+  - destruct l; ff.
+  - pps H1, H2. 
+    erewrite sorted_spec in H1, H2; ff.
+    pp (H0 H H5).
+    pp (H3 H6 H4).
+    clear H0 H3.
+    ltac1:(autorewrite with merge).
+    ff; neqbsimpl;
+    erewrite sorted_spec; split; ff.
+    * erewrite merge_in in *; ff a, l.
+    * erewrite merge_in in *; ff.
+      break_or_hyp.
+      + lia.
+      + eapply H1 in H0; ff l.
 Qed.
 
-Lemma perm_app_l : forall l l1 l2,
-  permutation l1 l2 ->
-  permutation (l ++ l1) (l ++ l2).
+Theorem merge_count : forall l1 l2 x,
+  count x (merge l1 l2) = count x (l1 ++ l2).
 Proof.
-  induction l; ff.
-  econstructor.
-  ff.
+  intros l1 l2.
+  pp (@list_sync_ind nat (fun lp => forall x : nat, count x (merge (fst lp) (snd lp)) = count x (fst lp ++ snd lp))).
+  simpl in *.
+  specialize H with (lp := (l1, l2)).
+  simpl in *.
+  eapply H; ff; clear H.
+  - destruct l. 
+    * ltac1:(autorewrite with merge in * ); ff.
+    * ltac1:(autorewrite with merge in * ); rewrite app_nil_r; ff.
+  - ltac1:(autorewrite with merge in * ); ff; neqbsimpl.
+    erewrite H0; ff;
+    repeat (erewrite count_app); ff l; neqbsimpl.
+  - ltac1:(autorewrite with merge in * ); ff; neqbsimpl;
+    erewrite H0; ff; neqbsimpl; ff;
+    repeat (erewrite count_app); ff l; neqbsimpl.
 Qed.
 
-Lemma perm_app : forall l1 l2 l3 l4,
-  permutation l1 l2 ->
-  permutation l3 l4 ->
-  permutation (l1 ++ l3) (l2 ++ l4).
-Proof.
-  intros.
-  prep_induction H.
-  induction H; ff.
-  - econstructor; ff.
-  - econstructor.
-    eapply perm_swap.
-    econstructor.
-    econstructor.
-    eapply perm_app_l.
-    ff.
-  - 
-    pp (IHpermutation1 l3 l4 H1).
-    pp (IHpermutation2 l4 l4 (perm_refl l4)).
-    eapply perm_trans; ff.
-Qed.
-
-Lemma perm_cons : forall l x,
-  permutation (x :: l) (l ++ x :: nil).
-Proof. 
-  induction l; ff.
-  - eapply perm_refl.
-  - eapply perm_trans with (l' := (a :: x :: l)).
-    * eapply perm_swap.
-    * econstructor; ff.
-Qed.
-
-Lemma perm_app_flip : forall l1 l2,
-  permutation (l1 ++ l2) (l2 ++ l1).
-Proof.
-  induction l1; ff.
-  - rewrite app_nil_r. eapply perm_refl.
-  - eapply perm_trans with (l' := (a :: (l2 ++ l1))).
-    * econstructor; ff.
-    * rewrite app_comm_cons.
-      assert (l2 ++ a :: l1 = (l2 ++ [a]) ++ l1). {
-        rewrite <- app_assoc.
-        ff.
-      }
-      rewrite H.
-      eapply perm_trans with (l' := ([a] ++ l2) ++ l1).
-      + simpl. eapply perm_refl.
-      + eapply perm_app > [ | eapply perm_refl ].
-        simpl.
-        eapply perm_trans.
-        eapply perm_cons.
-        eapply perm_refl.
-Qed.
-
-Lemma perm_app_cons : forall l1 l2 x,
-  permutation (l1 ++ x :: l2) (x :: l1 ++ l2).
-Proof.
-  intros.
-  rewrite app_comm_cons.
-  eapply perm_trans.
-  eapply perm_app_flip.
-  ff.
-  econstructor.
-  eapply perm_app_flip.
-Qed.
-
-Lemma perm_nil_iff_nil : forall l,
-  permutation nil l <-> l = nil.
-Proof.
-  split; ff.
-  - prep_induction H.
-    induction H; ff l.
-    erewrite IHpermutation2; ff.
-  - econstructor.
-Qed.
-
-Lemma perm_same_length : forall l1 l2,
-  permutation l1 l2 -> length l1 = length l2.
-Proof.
-  ff; induction H; ff l.
-Qed.
-
-Lemma count_in : forall l x,
-  count x l > 0 <-> In x l.
-Proof.
-  split; induction l; ff l; neqbsimpl; ff.
-Qed.
-
-Lemma same_count_same_length : forall l1 l2, 
-  (forall x : nat, count x l1 = count x l2) ->
-  length l1 = length l2.
-Proof.
-  assert (forall n, forall l1 l2, length l1 + length l2 < n -> 
-      (forall x : nat, count x l1 = count x l2) -> length l1 = length l2). {
-    induction n; ff l.
-
-    destruct l1, l2; ff l; neqbsimpl; ff.
-    - pp (H0 n0); ff l; neqbsimpl.
-    - pp (H0 n0); ff l; neqbsimpl.
-    - pp (H0 n0); pp (H0 n1); ff l; neqbsimpl.
-      * erewrite IHn; ff l; pp (H0 x); ff; neqbsimpl.
-      * 
-        assert (count n0 l2 > 0) by lia.
-        assert (count n1 l1 > 0) by lia.
-        erewrite count_in in *.
-        eapply in_split in H3.
-        eapply in_split in H4.
-        ff.
-        repeat (erewrite length_app in * ); ff l; neqbsimpl; ff.
-        f_equal.
-        repeat (erewrite count_app in * ); ff l; neqbsimpl; ff.
-        repeat (setoid_rewrite count_app in H0).
-        ff.
-        repeat (rewrite Nat.add_succ_r in * ).
-        repeat (rewrite <- length_app).
-        erewrite IHn; ff.
-        + repeat (erewrite length_app); ff l.
-        + repeat (erewrite count_app).
-          pp (H0 x3); ff l; neqbsimpl.
-  }
-  intros.
-  eapply H; ff l.
-Qed.
-
-Lemma count_permutation : forall l1 l2,
-  permutation l1 l2 <-> (forall x, count x l1 = count x l2).
-Proof.
-  split; ff.
-  - prep_induction H.
-    induction H; ff.
-  - 
-    (* ltac1:(generalize dependent H). *)
-    assert (forall n, forall l1 l2, length l1 + length l2 < n -> 
-        (forall x : nat, count x l1 = count x l2) -> permutation l1 l2). {
-      clear l1 l2 H.
-      induction n; ff l.
-    
-      destruct l1, l2; ff l; neqbsimpl; ff.
-      - econstructor.
-      - pp (H0 n0); ff l; neqbsimpl.
-      - pp (H0 n0); ff l; neqbsimpl.
-      - pp (H0 n0); pp (H0 n1); ff l; neqbsimpl.
-        * econstructor. eapply IHn; ff l; pp (H0 x); ff; neqbsimpl.
-        * 
-          assert (count n0 l2 > 0) by lia.
-          assert (count n1 l1 > 0) by lia.
-          erewrite count_in in *.
-          eapply in_split in H3.
-          eapply in_split in H4.
-          ff.
-          assert (permutation (x ++ x0) (x1 ++ x2)). {
-            eapply IHn; ff l.
-            repeat (rewrite length_app in * ).
-            ff l.
-            pp (H0 x3); ff; neqbsimpl;
-            repeat (rewrite count_app in * );
-            simpl in *; ff l; neqbsimpl; ff.
-          }
-          rewrite app_comm_cons.
-          rewrite app_comm_cons.
-          eapply perm_trans.
-          eapply perm_app_flip.
-          ff.
-          econstructor.
-          eapply perm_trans.
-          eapply perm_app_flip.
-          eapply perm_sym.
-          eapply perm_trans.
-          eapply perm_app_flip.
-          ff.
-          econstructor.
-          eapply perm_trans.
-          eapply perm_app_flip.
-          eapply perm_sym.
-          ff.
-    }
-    intros.
-    eapply H0; ff.
-Qed.
-
-
-(* Now we can define what it means for a sorting algorithm to be correct. *)
-Definition sort_correct (sort : list nat -> list nat) : Prop :=
-  forall l, 
-    (* The output of "sort" must be "sorted" *)
-    sorted (sort l) /\ 
-    (* The output of "sort" must have the same element counts as the input *)
-    (forall x, count x l = count x (sort l)).
-
-
-(** The Algorithms *)
-
-
-Module InsertionSort.
-
-  Fixpoint insert (x : nat) (l : list nat) : list nat :=
-    (* assumes l is already sorted *)
+Fixpoint split_at_n (l : list nat) (n : nat) : list nat * list nat :=
+  match n with
+  | 0 => (nil, l)
+  | S n' =>
     match l with
-    | nil => [x]
+    | nil => (nil, nil)
     | h :: t => 
-      (* find first place where x <= h, 
-        thus it can be safely inserted and maintain sortedness
-      *)
-      if x <=? h then
-        x :: l
-      else
-        h :: insert x t
-    end.
+      let '(l, r) := split_at_n t n' in
+      (h :: l, r)
+    end
+  end.
 
-  Lemma insert_sorted : forall x l,
-    sorted l ->
-    sorted (insert x l).
-  Proof.
-    intros.
-    prep_induction H.
-    induction H; ff; neqbsimpl; try (econstructor; ff l; fail).
-    - econstructor; ff l.
-      econstructor.
-    - econstructor; ff l.
-      econstructor.
-    - econstructor; ff.
-      pp (IHsorted x); ff; neqbsimpl.
-    - econstructor; ff l.
-      pp (IHsorted x0); ff; neqbsimpl.
-    - econstructor; ff l.
-      pp (IHsorted x0); ff; neqbsimpl.
-  Qed.
+Lemma split_at_n_zero : forall l,
+  snd (split_at_n l 0) = l.
+Proof.
+  destruct l; ff.
+Qed.
 
-  Lemma insert_count_cons : forall x y l,
-    count x (insert y l) = count x l + if Nat.eqb x y then 1 else 0.
-  Proof.
-    induction l; ff; neqbsimpl; ff.
-  Qed.
+Lemma split_at_n_length : forall l,
+  fst (split_at_n l (length l)) = l.
+Proof.
+  induction l; ff.
+Qed.
 
-  Fixpoint insertion_sort (l : list nat) : list nat :=
-    match l with
-    | nil => nil
-    | h :: t => insert h (insertion_sort t)
-    end.
+Lemma split_at_n_length_same : forall l n,
+  length (fst (split_at_n l n)) + length (snd (split_at_n l n)) = length l.
+Proof.
+  induction l; ff.
+  pp (IHl n0).
+  ff.
+Qed.
 
-  Theorem insertion_sort_correct : sort_correct insertion_sort.
-  Proof.
-    unfold sort_correct; split; ff.
-    - (* sortedness part *)
-      induction l; ff.
-      * econstructor.
-      * eapply insert_sorted; ff.
-    - (* counting part *)
-      induction l; ff; neqbsimpl; ff.
-      * erewrite insert_count_cons; ff l; neqbsimpl.
-      * erewrite insert_count_cons; ff l; neqbsimpl.
-  Qed.
+Lemma fst_split_at_n_length_lt : forall l n,
+  n < length l ->
+  length (fst (split_at_n l n)) = n.
+Proof.
+  induction l; ff l.
+  assert (n0 < length l) by lia.
+  eapply IHl in H0.
+  ff.
+Qed.
 
-End InsertionSort.
+Lemma snd_split_at_n_length_lt : forall l n,
+  n < length l ->
+  length (snd (split_at_n l n)) = length l - n.
+Proof.
+  induction l; ff l.
+  assert (n0 < length l) by lia.
+  eapply IHl in H0.
+  ff.
+Qed.
 
-Module MergeSort.
+Lemma split_at_n_rejoin : forall l n,
+  l = (fst (split_at_n l n) ++ snd (split_at_n l n)).
+Proof.
+  induction l; ff.
+  erewrite IHl; rewrite Heqp; ff.
+Qed.
 
-  Equations merge (l1 l2 : list nat) : list nat by wf (length l1 + length l2) :=
-    merge nil l2 := l2;
-    merge l1 nil := l1;
-    merge (h1 :: t1) (h2 :: t2) :=
-      if h1 <=? h2 
-      then h1 :: merge t1 (h2 :: t2)
-      else h2 :: merge (h1 :: t1) t2.
-  Next Obligation.
+Lemma add_n_div_n : forall n m,
+  0 < n ->
+  (n + m) / n = 1 + (m / n).
+Proof.
+  intros.
+  pp (Nat.div_add_l 1 n m).
+  simpl in *.
+  erewrite (Nat.add_0_r) in *.
+  ff l.
+Qed.
+
+Lemma n_div : forall n,
+  n / 2 < S n.
+Proof.
+  intros.
+  Search (_ / _ < _).
+  pp (Nat.div_lt (S n) 2).
+  (* assert (n / 2 <= S n / 2) by admit. *)
+  eapply Nat.lt_le_trans > [ | eapply H; lia ].
+  clear H.
+  pp (Nat.Div0.div_le_mono n (S n) 2).
+  assert (n <= S n) by lia.
+  eapply H in H0.
+  clear H.
+  lia.
+Qed.
+
+Show Obligation Tactic.
+Local Obligation Tactic := idtac.
+
+Equations merge_sort (l : list nat) : list nat by wf (length l) :=
+  merge_sort nil := nil;
+  merge_sort [h] := [h];
+  merge_sort v := 
+    merge (merge_sort (fst (split_at_n v (length v / 2)))) (merge_sort (snd (split_at_n v (length v / 2)))).
+Next Obligation.
+  intros.
+  subst v.
+  erewrite fst_split_at_n_length_lt.
+  - assert (length (n :: n0 :: l) = 2 + (length l)) by ff.
+    erewrite H.
+    erewrite add_n_div_n in *.
+    pp (n_div (length l)).
     lia.
-  Defined.
-
-  Program Fixpoint list_sync_ind {A : Type} (P : (list A * list A) -> Prop) 
-      (f_nil_l : forall r, P (nil, r))
-      (f_nil_r : forall l, P (l, nil))
-      (f_cons  : forall h1 h2 t1 t2, P (h1 :: t1, t2) /\ P (t1, h2 :: t2) -> P (h1 :: t1, h2 :: t2))
-      (lp : (list A * list A))
-      {measure (length (fst lp) + length (snd lp))}
-      : P lp :=
-    match lp with
-    | (nil, r) => f_nil_l r
-    | (l, nil) => f_nil_r l
-    | (h1 :: t1, h2 :: t2) => 
-      f_cons h1 h2 t1 t2 
-        (conj 
-          (list_sync_ind P f_nil_l f_nil_r f_cons (h1 :: t1, t2))
-          (list_sync_ind P f_nil_l f_nil_r f_cons (t1, h2 :: t2))
-        )
-    end.
-  Next Obligation.
     lia.
-  Qed.
-  Next Obligation.
-    eapply measure_wf.
-    eapply well_founded_ltof.
-  Qed.
-
-  Lemma merge_in : forall l1 l2 x,
-    In x (merge l1 l2) <-> In x l1 \/ In x l2.
-  Proof.
-    intros l1 l2.
-    pp (@list_sync_ind nat (fun lp => forall x : nat, In x (merge (fst lp) (snd lp)) <-> In x (fst lp) \/ In x (snd lp))).
-    simpl in *.
-    specialize H with (lp := (l1, l2)).
-    simpl in *.
-    eapply H; ff; clear H.
-    - ltac1:(autorewrite with merge in * ); destruct l; ff.
-    - ltac1:(autorewrite with merge in * ); destruct l; ff.
-    - ltac1:(autorewrite with merge in * ); ff.
-      * rewrite H1 in H; ff.
-      * rewrite H0 in H; ff.
-      Show Proof.
-      Print Assumptions merge_equation_3.
-    - ltac1:(autorewrite with merge in * ); ff.
-      * erewrite H1; ff.
-      * erewrite H0; ff.
-  Qed.
-  Print Assumptions merge_in.
-
-  Theorem merge_sorted : forall l1 l2,
-    sorted l1 ->
-    sorted l2 ->
-    sorted (merge l1 l2).
-  Proof.
-    intros l1 l2.
-    pp (@list_sync_ind nat (fun lp => sorted (fst lp) -> sorted (snd lp) -> sorted (merge (fst lp) (snd lp)))).
-    simpl in *.
-    specialize H with (lp := (l1, l2)).
-    simpl in *.
-    eapply H; ff; clear H.
-    - destruct l; ff.
-    - pps H1, H2. 
-      erewrite sorted_spec in H1, H2; ff.
-      pp (H0 H H5).
-      pp (H3 H6 H4).
-      clear H0 H3.
-      ltac1:(autorewrite with merge).
-      ff; neqbsimpl;
-      erewrite sorted_spec; split; ff.
-      * erewrite merge_in in *; ff a, l.
-      * erewrite merge_in in *; ff.
-        break_or_hyp.
-        + lia.
-        + eapply H1 in H0; ff l.
-  Qed.
-
-  Theorem merge_count : forall l1 l2 x,
-    count x (merge l1 l2) = count x (l1 ++ l2).
-  Proof.
-    intros l1 l2.
-    pp (@list_sync_ind nat (fun lp => forall x : nat, count x (merge (fst lp) (snd lp)) = count x (fst lp ++ snd lp))).
-    simpl in *.
-    specialize H with (lp := (l1, l2)).
-    simpl in *.
-    eapply H; ff; clear H.
-    - destruct l. 
-      * ltac1:(autorewrite with merge in * ); ff.
-      * ltac1:(autorewrite with merge in * ); rewrite app_nil_r; ff.
-    - ltac1:(autorewrite with merge in * ); ff; neqbsimpl.
-      erewrite H0; ff;
-      repeat (erewrite count_app); ff l; neqbsimpl.
-    - ltac1:(autorewrite with merge in * ); ff; neqbsimpl;
-      erewrite H0; ff; neqbsimpl; ff;
-      repeat (erewrite count_app); ff l; neqbsimpl.
-  Qed.
-
-  Fixpoint split_at_n (l : list nat) (n : nat) : list nat * list nat :=
-    match n with
-    | 0 => (nil, l)
-    | S n' =>
-      match l with
-      | nil => (nil, nil)
-      | h :: t => 
-        let '(l, r) := split_at_n t n' in
-        (h :: l, r)
-      end
-    end.
-
-  Lemma split_at_n_zero : forall l,
-    snd (split_at_n l 0) = l.
-  Proof.
-    destruct l; ff.
-  Qed.
-
-  Lemma split_at_n_length : forall l,
-    fst (split_at_n l (length l)) = l.
-  Proof.
-    induction l; ff.
-  Qed.
-
-  Lemma split_at_n_length_same : forall l n,
-    length (fst (split_at_n l n)) + length (snd (split_at_n l n)) = length l.
-  Proof.
-    induction l; ff.
-    pp (IHl n0).
-    ff.
-  Qed.
-
-  Lemma fst_split_at_n_length_lt : forall l n,
-    n < length l ->
-    length (fst (split_at_n l n)) = n.
-  Proof.
-    induction l; ff l.
-    assert (n0 < length l) by lia.
-    eapply IHl in H0.
-    ff.
-  Qed.
-
-  Lemma snd_split_at_n_length_lt : forall l n,
-    n < length l ->
-    length (snd (split_at_n l n)) = length l - n.
-  Proof.
-    induction l; ff l.
-    assert (n0 < length l) by lia.
-    eapply IHl in H0.
-    ff.
-  Qed.
-
-  Lemma split_at_n_rejoin : forall l n,
-    l = (fst (split_at_n l n) ++ snd (split_at_n l n)).
-  Proof.
-    induction l; ff.
-    erewrite IHl; rewrite Heqp; ff.
-  Qed.
-
-  Lemma add_n_div_n : forall n m,
-    0 < n ->
-    (n + m) / n = 1 + (m / n).
-  Proof.
-    intros.
-    pp (Nat.div_add_l 1 n m).
-    simpl in *.
-    erewrite (Nat.add_0_r) in *.
-    ff l.
-  Qed.
-
-  Lemma n_div : forall n,
-    n / 2 < S n.
-  Proof.
-    intros.
-    Search (_ / _ < _).
-    pp (Nat.div_lt (S n) 2).
-    (* assert (n / 2 <= S n / 2) by admit. *)
-    eapply Nat.lt_le_trans > [ | eapply H; lia ].
-    clear H.
-    pp (Nat.Div0.div_le_mono n (S n) 2).
-    assert (n <= S n) by lia.
-    eapply H in H0.
-    clear H.
+  - assert (length (n :: n0 :: l) = 2 + (length l)) by ff.
+    erewrite H.
+    erewrite add_n_div_n in *.
+    pp (n_div (length l)).
     lia.
-  Qed.
+    lia.
+Defined.
+Next Obligation.
+  intros.
+  subst v.
+  erewrite snd_split_at_n_length_lt.
+  - assert (length (n :: n0 :: l) = 2 + (length l)) by ff.
+    erewrite H.
+    erewrite add_n_div_n in *.
+    pp (n_div (length l)).
+    lia.
+    lia.
+  - assert (length (n :: n0 :: l) = 2 + (length l)) by ff.
+    erewrite H.
+    erewrite add_n_div_n in *.
+    pp (n_div (length l)).
+    lia.
+    lia.
+Defined.
 
-  Show Obligation Tactic.
-  Local Obligation Tactic := idtac.
-
-  Equations merge_sort (l : list nat) : list nat by wf (length l) :=
-    merge_sort nil := nil;
-    merge_sort [h] := [h];
-    merge_sort v := 
-      merge (merge_sort (fst (split_at_n v (length v / 2)))) (merge_sort (snd (split_at_n v (length v / 2)))).
-  Next Obligation.
-    intros.
-    subst v.
-    erewrite fst_split_at_n_length_lt.
-    - assert (length (n :: n0 :: l) = 2 + (length l)) by ff.
-      erewrite H.
-      erewrite add_n_div_n in *.
-      pp (n_div (length l)).
-      lia.
-      lia.
-    - assert (length (n :: n0 :: l) = 2 + (length l)) by ff.
-      erewrite H.
-      erewrite add_n_div_n in *.
-      pp (n_div (length l)).
-      lia.
-      lia.
-  Defined.
-  Next Obligation.
-    intros.
-    subst v.
-    erewrite snd_split_at_n_length_lt.
-    - assert (length (n :: n0 :: l) = 2 + (length l)) by ff.
-      erewrite H.
-      erewrite add_n_div_n in *.
-      pp (n_div (length l)).
-      lia.
-      lia.
-    - assert (length (n :: n0 :: l) = 2 + (length l)) by ff.
-      erewrite H.
-      erewrite add_n_div_n in *.
-      pp (n_div (length l)).
-      lia.
-      lia.
-  Defined.
-
-  Theorem merge_sort_correct : sort_correct merge_sort.
-  Proof.
-    unfold sort_correct; split; ff.
-    - (* sorting part *)
-      (* here is a hacky way to get strong induction! *)
-      assert (forall n : nat, forall l : list nat, length l < n -> sorted (merge_sort l)). {
-        clear l.
-        induction n; ff.
-        - destruct l; ff l.
-        - destruct l.
-          * ltac1:(autorewrite with merge_sort).
+Theorem merge_sort_correct : sort_correct merge_sort.
+Proof.
+  unfold sort_correct; split; ff.
+  - (* sorting part *)
+    (* here is a hacky way to get strong induction! *)
+    assert (forall n : nat, forall l : list nat, length l < n -> sorted (merge_sort l)). {
+      clear l.
+      induction n; ff.
+      - destruct l; ff l.
+      - destruct l.
+        * ltac1:(autorewrite with merge_sort).
+          econstructor.
+        * destruct l.
+          ** ltac1:(autorewrite with merge_sort).
             econstructor.
-          * destruct l.
-            ** ltac1:(autorewrite with merge_sort).
-              econstructor.
-            ** ltac1:(autorewrite with merge_sort).
-              eapply merge_sorted; eapply IHn.
-              (* Some non-trivial (but definitely true) arithmetic stuff *)
-              + erewrite fst_split_at_n_length_lt.
-                -- assert (length (n0 :: n1 :: l) = 2 + (length l)) by ff.
-                    erewrite H0.
-                    erewrite add_n_div_n in *.
-                    pp (n_div (length l)).
-                    lia.
-                    lia.
-                -- assert (length (n0 :: n1 :: l) = 2 + (length l)) by ff.
-                    erewrite H0.
-                    erewrite add_n_div_n in *.
-                    pp (n_div (length l)).
-                    lia.
-                    lia.
-              + erewrite snd_split_at_n_length_lt.
-                -- assert (length (n0 :: n1 :: l) = 2 + (length l)) by ff.
+          ** ltac1:(autorewrite with merge_sort).
+            eapply merge_sorted; eapply IHn.
+            (* Some non-trivial (but definitely true) arithmetic stuff *)
+            + erewrite fst_split_at_n_length_lt.
+              -- assert (length (n0 :: n1 :: l) = 2 + (length l)) by ff.
                   erewrite H0.
                   erewrite add_n_div_n in *.
                   pp (n_div (length l)).
                   lia.
                   lia.
-                -- assert (length (n0 :: n1 :: l) = 2 + (length l)) by ff.
+              -- assert (length (n0 :: n1 :: l) = 2 + (length l)) by ff.
                   erewrite H0.
                   erewrite add_n_div_n in *.
                   pp (n_div (length l)).
                   lia.
                   lia.
-      }
-      eapply H with (n := S (length l)).
-      lia.
-    - (* counting part *)
-      assert (forall n : nat, forall x l, length l < n -> count x l = count x (merge_sort l)). {
-        clear x l.
-        induction n; ff.
-        - destruct l; ff l.
-        - destruct l.
-          * ltac1:(autorewrite with merge_sort).
+            + erewrite snd_split_at_n_length_lt.
+              -- assert (length (n0 :: n1 :: l) = 2 + (length l)) by ff.
+                erewrite H0.
+                erewrite add_n_div_n in *.
+                pp (n_div (length l)).
+                lia.
+                lia.
+              -- assert (length (n0 :: n1 :: l) = 2 + (length l)) by ff.
+                erewrite H0.
+                erewrite add_n_div_n in *.
+                pp (n_div (length l)).
+                lia.
+                lia.
+    }
+    eapply H with (n := S (length l)).
+    lia.
+  - (* counting part *)
+    assert (forall n : nat, forall x l, length l < n -> count x l = count x (merge_sort l)). {
+      clear x l.
+      induction n; ff.
+      - destruct l; ff l.
+      - destruct l.
+        * ltac1:(autorewrite with merge_sort).
+          econstructor.
+        * destruct l.
+          ** ltac1:(autorewrite with merge_sort).
             econstructor.
-          * destruct l.
-            ** ltac1:(autorewrite with merge_sort).
-              econstructor.
-            ** ltac1:(autorewrite with merge_sort).
-              erewrite merge_count.
-              erewrite count_app.
-              repeat (erewrite <- IHn).
-              erewrite <- count_app.
-              pp (split_at_n_rejoin (n0 :: n1 :: l)).
-              erewrite <- H0; ff.
-              (* Same non-trivial arith as above *)
-              + erewrite snd_split_at_n_length_lt.
-                -- assert (length (n0 :: n1 :: l) = 2 + (length l)) by ff.
+          ** ltac1:(autorewrite with merge_sort).
+            erewrite merge_count.
+            erewrite count_app.
+            repeat (erewrite <- IHn).
+            erewrite <- count_app.
+            pp (split_at_n_rejoin (n0 :: n1 :: l)).
+            erewrite <- H0; ff.
+            (* Same non-trivial arith as above *)
+            + erewrite snd_split_at_n_length_lt.
+              -- assert (length (n0 :: n1 :: l) = 2 + (length l)) by ff.
+                erewrite H0.
+                erewrite add_n_div_n in *.
+                pp (n_div (length l)).
+                lia.
+                lia.
+              -- assert (length (n0 :: n1 :: l) = 2 + (length l)) by ff.
+                erewrite H0.
+                erewrite add_n_div_n in *.
+                pp (n_div (length l)).
+                lia.
+                lia.
+            + erewrite fst_split_at_n_length_lt.
+              -- assert (length (n0 :: n1 :: l) = 2 + (length l)) by ff.
                   erewrite H0.
                   erewrite add_n_div_n in *.
                   pp (n_div (length l)).
                   lia.
                   lia.
-                -- assert (length (n0 :: n1 :: l) = 2 + (length l)) by ff.
+              -- assert (length (n0 :: n1 :: l) = 2 + (length l)) by ff.
                   erewrite H0.
                   erewrite add_n_div_n in *.
                   pp (n_div (length l)).
                   lia.
                   lia.
-             + erewrite fst_split_at_n_length_lt.
-                -- assert (length (n0 :: n1 :: l) = 2 + (length l)) by ff.
-                    erewrite H0.
-                    erewrite add_n_div_n in *.
-                    pp (n_div (length l)).
-                    lia.
-                    lia.
-                -- assert (length (n0 :: n1 :: l) = 2 + (length l)) by ff.
-                    erewrite H0.
-                    erewrite add_n_div_n in *.
-                    pp (n_div (length l)).
-                    lia.
-                    lia.
-      }
-      eapply H with (n := S (length l)).
-      lia.
-  Qed.
+    }
+    eapply H with (n := S (length l)).
+    lia.
+Qed.
 
-  Print Assumptions merge_sort_correct.
-
-End MergeSort.
-
-
-Module BubbleSort.
-
-  (*
-
-  Local Obligation Tactic := 
-    simpl in *; Tactics.program_simplify;
-    CoreTactics.equations_simpl;
-    try Tactics.program_solve_wf.
-
-  Program Fixpoint list_ind_two {A : Type} (P : list A -> Prop) 
-      (fnil : P nil)
-      (fsingle : forall x, P [x]) 
-      (fcons_two : forall x y l, P (x :: l) /\ P (y :: l) -> P (cons x (cons y l))) (l : list A) {measure (length l)} : P l :=
-    match l with
-    | nil => fnil
-    | [x] => fsingle x
-    | x :: y :: l => 
-      fcons_two x y l (conj 
-        (list_ind_two P fnil fsingle fcons_two (x :: l)) 
-        (list_ind_two P fnil fsingle fcons_two (y :: l)))
-    end.
-  Next Obligation.
-    eapply measure_wf.
-    eapply well_founded_ltof.
-  Qed.
-
-  Equations bubble_up (l : list nat) : list nat by wf (length l) :=
-  bubble_up nil := nil;
-  bubble_up (cons x nil) := (cons x nil);
-  bubble_up (cons x (cons y t)) :=
-        (* x < y, so we are good *)
-        if Nat.leb x y then
-          x :: bubble_up (y :: t)
-        else
-          (* x >= y, so we need to swap *)
-          y :: bubble_up (x :: t).
-
-  Ltac2 Notation "neqbsimpl" :=
-    try (rewrite Nat.eqb_eq in * ); ff;
-    try (rewrite Nat.eqb_neq in * ); ff;
-    try (rewrite Nat.ltb_irrefl in * ); ff.
-
-  Lemma bubble_up_count_invariant : forall l, 
-    forall x, count x l = count x (bubble_up l).
-  Proof.
-    induction l using @list_ind_two; intros.
-    - ltac1:(autorewrite with bubble_up); ff.
-    - ltac1:(autorewrite with bubble_up); ff.
-    - ltac1:(autorewrite with bubble_up); ff;
-      neqbsimpl.
-      all: try (rewrite <- H; ff; neqbsimpl).
-      all: try (rewrite <- H0; ff; neqbsimpl).
-  Qed.
-
-  Lemma bubble_up_in_same : forall l,
-    forall x, In x l <-> In x (bubble_up l).
-  Proof.
-    induction l using @list_ind_two; intros.
-    - ltac1:(autorewrite with bubble_up); ff.
-    - ltac1:(autorewrite with bubble_up); ff.
-    - ltac1:(autorewrite with bubble_up); ff;
-      neqbsimpl.
-      all: try (rewrite <- H in *; ff; neqbsimpl).
-      all: try (rewrite <- H0 in *; ff; neqbsimpl).
-  Qed.
-
-  Fixpoint min (l : list nat) : option nat :=
-    match l with
-    | nil => None
-    | h :: t =>
-      match min t with
-      | None => Some h
-      | Some v => Some (Nat.min h v)
-      end
-    end.
-
-  Lemma bubble_up_sorted_invariant : forall l,
-    sorted l ->
-    sorted (bubble_up l).
-  Proof.
-    induction l using @list_ind_two; ff.
-    ltac1:(autorewrite with bubble_up).
-    invc H0.
-    pp (H1 H6).
-    erewrite <- Nat.leb_le in *.
-    ff.
-    clear H H1.
-    erewrite sorted_spec in *; ff.
-    split; ff.
-    erewrite Nat.leb_le in *.
-    erewrite H4.
-    clear H4.
-    erewrite <- bubble_up_in_same in *.
-    simpl in *; ff.
-  Qed.
-
-  Lemma bubble_up_sorted_cons : forall l,
-    sorted l ->
-    forall h, sorted (bubble_up (h :: l)).
-  Proof.
-    induction l using @list_ind_two; ff.
-    - ltac1:(autorewrite with bubble_up); econstructor.
-    - ltac1:(autorewrite with bubble_up); ff; econstructor;
-      neqbsimpl; ff.
-      * erewrite Nat.leb_le in *; ff.
-      * erewrite Nat.leb_gt in *; ff l.
-      * econstructor.
-    - ltac1:(autorewrite with bubble_up).
-      invc H0.
-      pp (H1 H6).
-      erewrite <- Nat.leb_le in *.
-      ff; clear H H1;
-      erewrite Nat.leb_le in *.
-      * erewrite sorted_spec in *; ff.
-        split; ff l.
-        + admit.
-        + admit.
-    
-
-  Compute (bubble_up [3;2;1]).
-
-  (* Now, we need to do n passes of the bubble-up procedure! *)
-
-  Fixpoint do_n_times {A : Type} (f : A -> A) (l : A) (n : nat) : A :=
-    match n with
-    | 0 => l
-    | S n' => f (do_n_times f l n')
-    end.
-
-  Lemma do_n_times_invariants : forall {A : Type} (P : A -> Prop) f a n,
-    (forall a', P a' -> P (f a')) ->
-    P a ->
-    P (do_n_times f a n).
-  Proof.
-    induction n; ff.
-  Qed.
-
-  Definition bubble_sort (l : list nat) : list nat :=
-    do_n_times bubble_up l (length l).
-
-  Example test1 : bubble_sort [3;2;1;0] = [0;1;2;3].
-  Proof. reflexivity. Qed.
-
-  Example test2 : bubble_sort [5;1;4;2;8] = [1;2;4;5;8].
-  Proof. reflexivity. Qed.
-
-  Example test3 : bubble_sort [3;3;2;1;4;4] = [1;2;3;3;4;4].
-  Proof. reflexivity. Qed.
-
-  (* Now, time to prove correctness! *)
-
-  Theorem bubble_sort_correct : sort_correct bubble_sort.
-  Proof.
-    unfold sort_correct; intros.
-    split.
-    - (* is it sorted! *)
-      induction l; unfold bubble_sort in *; simpl.
-      * econstructor.
-      * eapply do_n_times_invariants.
-        admit.
-        admit.
-    - (* does it have the same counts! *)
-      unfold bubble_sort.
-      eapply do_n_times_invariants; ff.
-      erewrite H.
-      eapply bubble_up_count_invariant.
-
-  *)
-End BubbleSort.
+Print Assumptions merge_sort_correct.
