BubbleSort.v
@@ -1,0 +1,166 @@
+(*
+
+Local Obligation Tactic := 
+  simpl in *; Tactics.program_simplify;
+  CoreTactics.equations_simpl;
+  try Tactics.program_solve_wf.
+
+Program Fixpoint list_ind_two {A : Type} (P : list A -> Prop) 
+    (fnil : P nil)
+    (fsingle : forall x, P [x]) 
+    (fcons_two : forall x y l, P (x :: l) /\ P (y :: l) -> P (cons x (cons y l))) (l : list A) {measure (length l)} : P l :=
+  match l with
+  | nil => fnil
+  | [x] => fsingle x
+  | x :: y :: l => 
+    fcons_two x y l (conj 
+      (list_ind_two P fnil fsingle fcons_two (x :: l)) 
+      (list_ind_two P fnil fsingle fcons_two (y :: l)))
+  end.
+Next Obligation.
+  eapply measure_wf.
+  eapply well_founded_ltof.
+Qed.
+
+Equations bubble_up (l : list nat) : list nat by wf (length l) :=
+bubble_up nil := nil;
+bubble_up (cons x nil) := (cons x nil);
+bubble_up (cons x (cons y t)) :=
+      (* x < y, so we are good *)
+      if Nat.leb x y then
+        x :: bubble_up (y :: t)
+      else
+        (* x >= y, so we need to swap *)
+        y :: bubble_up (x :: t).
+
+Ltac2 Notation "neqbsimpl" :=
+  try (rewrite Nat.eqb_eq in * ); ff;
+  try (rewrite Nat.eqb_neq in * ); ff;
+  try (rewrite Nat.ltb_irrefl in * ); ff.
+
+Lemma bubble_up_count_invariant : forall l, 
+  forall x, count x l = count x (bubble_up l).
+Proof.
+  induction l using @list_ind_two; intros.
+  - ltac1:(autorewrite with bubble_up); ff.
+  - ltac1:(autorewrite with bubble_up); ff.
+  - ltac1:(autorewrite with bubble_up); ff;
+    neqbsimpl.
+    all: try (rewrite <- H; ff; neqbsimpl).
+    all: try (rewrite <- H0; ff; neqbsimpl).
+Qed.
+
+Lemma bubble_up_in_same : forall l,
+  forall x, In x l <-> In x (bubble_up l).
+Proof.
+  induction l using @list_ind_two; intros.
+  - ltac1:(autorewrite with bubble_up); ff.
+  - ltac1:(autorewrite with bubble_up); ff.
+  - ltac1:(autorewrite with bubble_up); ff;
+    neqbsimpl.
+    all: try (rewrite <- H in *; ff; neqbsimpl).
+    all: try (rewrite <- H0 in *; ff; neqbsimpl).
+Qed.
+
+Fixpoint min (l : list nat) : option nat :=
+  match l with
+  | nil => None
+  | h :: t =>
+    match min t with
+    | None => Some h
+    | Some v => Some (Nat.min h v)
+    end
+  end.
+
+Lemma bubble_up_sorted_invariant : forall l,
+  sorted l ->
+  sorted (bubble_up l).
+Proof.
+  induction l using @list_ind_two; ff.
+  ltac1:(autorewrite with bubble_up).
+  invc H0.
+  pp (H1 H6).
+  erewrite <- Nat.leb_le in *.
+  ff.
+  clear H H1.
+  erewrite sorted_spec in *; ff.
+  split; ff.
+  erewrite Nat.leb_le in *.
+  erewrite H4.
+  clear H4.
+  erewrite <- bubble_up_in_same in *.
+  simpl in *; ff.
+Qed.
+
+Lemma bubble_up_sorted_cons : forall l,
+  sorted l ->
+  forall h, sorted (bubble_up (h :: l)).
+Proof.
+  induction l using @list_ind_two; ff.
+  - ltac1:(autorewrite with bubble_up); econstructor.
+  - ltac1:(autorewrite with bubble_up); ff; econstructor;
+    neqbsimpl; ff.
+    * erewrite Nat.leb_le in *; ff.
+    * erewrite Nat.leb_gt in *; ff l.
+    * econstructor.
+  - ltac1:(autorewrite with bubble_up).
+    invc H0.
+    pp (H1 H6).
+    erewrite <- Nat.leb_le in *.
+    ff; clear H H1;
+    erewrite Nat.leb_le in *.
+    * erewrite sorted_spec in *; ff.
+      split; ff l.
+      + admit.
+      + admit.
+  
+
+Compute (bubble_up [3;2;1]).
+
+(* Now, we need to do n passes of the bubble-up procedure! *)
+
+Fixpoint do_n_times {A : Type} (f : A -> A) (l : A) (n : nat) : A :=
+  match n with
+  | 0 => l
+  | S n' => f (do_n_times f l n')
+  end.
+
+Lemma do_n_times_invariants : forall {A : Type} (P : A -> Prop) f a n,
+  (forall a', P a' -> P (f a')) ->
+  P a ->
+  P (do_n_times f a n).
+Proof.
+  induction n; ff.
+Qed.
+
+Definition bubble_sort (l : list nat) : list nat :=
+  do_n_times bubble_up l (length l).
+
+Example test1 : bubble_sort [3;2;1;0] = [0;1;2;3].
+Proof. reflexivity. Qed.
+
+Example test2 : bubble_sort [5;1;4;2;8] = [1;2;4;5;8].
+Proof. reflexivity. Qed.
+
+Example test3 : bubble_sort [3;3;2;1;4;4] = [1;2;3;3;4;4].
+Proof. reflexivity. Qed.
+
+(* Now, time to prove correctness! *)
+
+Theorem bubble_sort_correct : sort_correct bubble_sort.
+Proof.
+  unfold sort_correct; intros.
+  split.
+  - (* is it sorted! *)
+    induction l; unfold bubble_sort in *; simpl.
+    * econstructor.
+    * eapply do_n_times_invariants.
+      admit.
+      admit.
+  - (* does it have the same counts! *)
+    unfold bubble_sort.
+    eapply do_n_times_invariants; ff.
+    erewrite H.
+    eapply bubble_up_count_invariant.
+
+*)
